\documentclass{article}
\usepackage[utf8]{inputenc}
\usepackage{geometry} 
\usepackage{amsmath}  
\usepackage{graphicx} 

\begin{document}
\begin{align*}
\text{1.Calcula}\\
&\lim_{n \to \infty}\frac{n^3+2n-1}{5n^3+n^2-2n+1}=\frac{1}{5}\\
\text{2.Calcula}\\
&\lim_{x \to \infty}\sqrt{n^2-n}-\sqrt{n^2+4n}=\frac{-5}{2}\\
\text{3.Calcula}\\
&\lim_{x \to \infty}\ln(1+n+\sqrt{n})-\ln(n)=0\\
\text{4.Calcula}\\
&\lim_{x \to \infty}\frac{1^3+2^3+\cdots+n^3}{n^4}=\frac{1}{4} \\
\text{5.Calcula}\\
&\lim_{x \to \infty}{\left(\frac{n^3-2n}{n^3+3n^2-2n-1}\right)}^n=e^{(-3)}  \\
\text{6.Calcula}\\
&\sum_{n = 2}^{\infty}\frac{n+2}{n^3-n}=\frac{5}{4} \\
\text{7.Calcula}\\
&\sum_{n = 2}^{\infty}\frac{1}{n^3-n}=\frac{1}{4} \\
\text{8.Calcula}\\
&\sum_{n = 0}^{\infty}{(-1)}^n{x^n}={-1}^n\sum_{n = 0}^{\infty}x^{n}  \\
\text{9.Calcula}\\
&\sum_{n = 0}^{\infty}{(-1)}^n{4^n}{x^{2n}}=4^n{(-1)}^{n}\sum_{n = 0}^{\infty}x^{2n}  \\
\text{10.Calcula la serie de Taylor en el orígen de la funcion}\\
&f{(x)}=\frac{1}{1+x^2}=-8x^3+4x^2-2x+1\\
\text{11.Calcula la serie de Taylor en el orígen de la funcion}\\
&g{(x)}=x\cos(x)=\frac{-1}{2}x^3+x 
\end{align*}

\end{document}
